KMcK

Foundation/Modal/Entailment/Basic.lean
@@ -631,10 +631,10 @@ instance [Entailment.Triv 𝓢] : Entailment.KTc 𝓢 where
 
 protected class Ver extends Entailment.K 𝓢, HasAxiomVer 𝓢
 
-protected class KM extends Entailment.K 𝓢, HasAxiomMcK 𝓢
+protected class KMcK extends Entailment.K 𝓢, HasAxiomMcK 𝓢
 
 protected class K4 extends Entailment.K 𝓢, HasAxiomFour 𝓢
-protected class K4M extends Entailment.K4 𝓢, HasAxiomMcK 𝓢
+protected class K4McK extends Entailment.K4 𝓢, HasAxiomMcK 𝓢
 protected class K4Point2 extends Entailment.K4 𝓢, HasAxiomWeakPoint2 𝓢
 protected class K4Point3 extends Entailment.K4 𝓢, HasAxiomWeakPoint3 𝓢
 protected class KD4Point3Z extends Entailment.K 𝓢, HasAxiomD 𝓢, HasAxiomFour 𝓢, HasAxiomWeakPoint3 𝓢, HasAxiomZ 𝓢
@@ -648,10 +648,10 @@ instance [Entailment.S4 𝓢] : Entailment.KT 𝓢 where
 protected class S4Point2 extends Entailment.S4 𝓢, HasAxiomPoint2 𝓢
 protected class S4Point3 extends Entailment.S4 𝓢, HasAxiomPoint3 𝓢
 protected class S4Point4 extends Entailment.S4 𝓢, HasAxiomPoint4 𝓢
-protected class S4M extends Entailment.S4 𝓢, HasAxiomMcK 𝓢
-protected class S4Point2M extends Entailment.S4M 𝓢, HasAxiomPoint2 𝓢
-protected class S4Point3M extends Entailment.S4M 𝓢, HasAxiomPoint3 𝓢
-protected class S4Point4M extends Entailment.S4M 𝓢, HasAxiomPoint4 𝓢
+protected class S4McK extends Entailment.S4 𝓢, HasAxiomMcK 𝓢
+protected class S4Point2McK extends Entailment.S4McK 𝓢, HasAxiomPoint2 𝓢
+protected class S4Point3McK extends Entailment.S4McK 𝓢, HasAxiomPoint3 𝓢
+protected class S4Point4McK extends Entailment.S4McK 𝓢, HasAxiomPoint4 𝓢
 
 protected class S5 extends Entailment.K 𝓢, HasAxiomT 𝓢, HasAxiomFive 𝓢
 instance [Entailment.S5 𝓢] : Entailment.KT 𝓢 where
